cedar-lean/Cedar/TPE/BatchedEvaluator.lean
@@ -1,0 +1,83 @@
+/-
+ Copyright Cedar Contributors
+
+ Licensed under the Apache License, Version 2.0 (the "License");
+ you may not use this file except in compliance with the License.
+ You may obtain a copy of the License at
+
+      https://www.apache.org/licenses/LICENSE-2.0
+
+ Unless required by applicable law or agreed to in writing, software
+ distributed under the License is distributed on an "AS IS" BASIS,
+ WITHOUT WARRANTIES OR CONDITIONS OF ANY KIND, either express or implied.
+ See the License for the specific language governing permissions and
+ limitations under the License.
+-/
+
+
+import Cedar.Spec
+import Cedar.Data
+import Cedar.TPE.Residual
+import Cedar.TPE.Evaluator
+import Cedar.TPE.Input
+
+namespace Cedar.TPE
+
+open Cedar.Data
+open Cedar.Spec
+open Cedar.Validation
+
+
+abbrev EntityLoader := Set EntityUID → Map EntityUID PartialEntityData
+
+/--
+The batched evaluation loop
+  1. Asks for any new entities referenced by the residual
+  2. Partially evaluates now that new entities are loaded
+  3. Exits if a value has been found
+-/
+partial def batchedEvalLoop
+  (residual : Residual)
+  (req : Request)
+  (loader : EntityLoader)
+  (store : PartialEntities)
+  : Result Value :=
+  let toLoad := residual.allLiteralUIDs.filter (λ uid => (store.find? uid).isNone)
+  let newEntities := loader toLoad
+  let newStore := newEntities ++ store
+  let newRes := Cedar.TPE.evaluate residual req.asPartialRequest newStore
+
+  match newRes with
+  | .val v _ty => .ok v
+  | _ => batchedEvalLoop newRes req loader newStore
+
+
+/--
+Evaluate a cedar expression using an EntityLoader
+instead of a full Entities store.
+This algorithm minimizes the number of calls to the EntityLoader using partial evaluation.
+-/
+def batchedEvaluate
+  (x : TypedExpr)
+  (req : Request)
+  (loader : EntityLoader)
+  : Result Value :=
+  let residual := Cedar.TPE.evaluate x.toResidual req.asPartialRequest Map.empty
+  -- start the batched evaluation loop
+  batchedEvalLoop residual req loader Map.empty
+
+/--
+Create an entity loader for an entity store Entities.
+This is used to model user-provided entity loaders which
+load entities from a backing database.
+
+Given Entities es, the entity loader provides the requested
+entities specified by a set of entity ids.
+-/
+def entityLoaderFor (es: Entities) (uids : Set EntityUID) :=
+  Map.make (uids.toList.map (λ uid =>
+        match (es.find? uid) with
+        | .some data =>
+          (uid, data.asPartial)
+        | .none =>
+          (uid, PartialEntityData.absent)))
